examples/wysteria/sinterpreter.fst
@@ -1,13 +1,13 @@
 (*--build-config
-    options:--admit_fsi OrdSet --admit_fsi OrdMap --admit_fsi Set --admit_fsi FFI;
+    options:--admit_fsi FStar.OrdSet --admit_fsi FStar.OrdMap --admit_fsi Set --admit_fsi FFI;
     variables:LIB=../../lib;
     other-files:set.fsi $LIB/ordset.fsi $LIB/ordmap.fsi $LIB/classical.fst ast.fst ffi.fsi sem.fst
  --*)
 
 module SourceInterpreter
 
-open OrdMap
-open OrdSet
+open FStar.OrdMap
+open FStar.OrdSet
 
 open AST
 
@@ -37,7 +37,7 @@ let step c =
   else if is_value c && is_sframe c is_F_ffi then Some (step_ffi_l c)
   else if is_value c && is_sframe c is_F_match then Some (step_match_red c)
   else if is_value c && is_sframe c is_F_aspar_e then Some (step_aspar_red c)
-  else if is_value c && is_sframe c is_F_box_e then Some (step_box_red c)
+  //else if is_value c && is_sframe c is_F_box_e then Some (step_box_red c)
   else if is_value c && is_sframe c is_F_unbox then Some (step_unbox_red c)
   else if is_value c && is_sframe c is_F_mkwire_e then Some (step_mkwire_red c)
   else if is_value c && is_sframe c is_F_projwire_e then Some (step_projwire_red c)
@@ -49,11 +49,12 @@ let step c =
   else if pre_ffi c = Do then Some (step_ffi c)
   else if pre_match c = Do then Some (step_match c)
   else if not (pre_aspar c = NA) then Some (step_aspar c)
-  else if pre_box c = Do then Some (step_box c)
+  //else if pre_box c = Do then Some (step_box c)
   else if pre_unbox c = Do then Some (step_unbox c)
   else if pre_mkwire c = Do then Some (step_mkwire c)
   else if pre_projwire c = Do then Some (step_projwire c)
   else if pre_concatwire c = Do then Some (step_concatwire c)
+  else if pre_aspar_ret c = Do then Some (step_aspar_ret c)
   else if pre_eassec c then Some (step_assec_e1 c)
   else if is_value_ps c && is_sframe c is_F_assec_ps then Some (step_assec_e2 c)
   else if is_value c && is_sframe c is_F_assec_e then Some (step_assec_red c)
@@ -87,7 +88,7 @@ let step_correctness c =
   else if is_value c && is_sframe c is_F_ffi then C_ffi_l c c'
   else if is_value c && is_sframe c is_F_match then C_match_red c c'
   else if is_value c && is_sframe c is_F_aspar_e then C_aspar_red c c'
-  else if is_value c && is_sframe c is_F_box_e then C_box_red c c'
+  //else if is_value c && is_sframe c is_F_box_e then C_box_red c c'
   else if is_value c && is_sframe c is_F_unbox then C_unbox_red c c'
   else if is_value c && is_sframe c is_F_mkwire_e then C_mkwire_red c c'
   else if is_value c && is_sframe c is_F_projwire_e then C_projwire_red c c'
@@ -99,11 +100,12 @@ let step_correctness c =
   else if pre_ffi c = Do then C_ffi_beta c c'
   else if pre_match c = Do then C_match_beta c c'
   else if not (pre_aspar c = NA) then C_aspar_beta c c'
-  else if pre_box c = Do then C_box_beta c c'
+  //else if pre_box c = Do then C_box_beta c c'
   else if pre_unbox c = Do then C_unbox_beta c c'
   else if pre_mkwire c = Do then C_mkwire_beta c c'
   else if pre_projwire c = Do then C_projwire_beta c c'
   else if pre_concatwire c = Do then C_concatwire_beta c c'
+  else if pre_aspar_ret c = Do then C_aspar_ret c c'
   else if pre_eassec c then C_assec_ps c c'
   else if is_value_ps c && is_sframe c is_F_assec_ps then C_assec_e c c'
   else if is_value c && is_sframe c is_F_assec_e then C_assec_red c c'
